HOL/SepLogic/Quicksort.thy
@@ -1,6 +1,5 @@
 theory Quicksort
-imports Reverse More_Lists
-  "~~/src/HOL/Imperative_HOL/ex/Subarray"
+imports Reverse "../DataStrs/Quicksort_Func2"
 begin
 
 function part1 :: "nat array \<Rightarrow> nat \<Rightarrow> nat \<Rightarrow> nat \<Rightarrow> nat Heap"
@@ -14,9 +13,8 @@ where
         else (do { swap a left right;
                    part1 a left (right - 1) p }))
      })"
-by pat_completeness auto termination by (relation "measure (\<lambda>(_,l,r,_). r - l )") auto
-
-declare part1.simps [sep_proc_defs]
+  by auto
+  termination by (relation "measure (\<lambda>(_,l,r,_). r - l )") auto
 
 theorem part1_induct': "(\<forall>a left right p.
     ((\<not> right \<le> left \<longrightarrow> (\<forall>v.  v \<le> p \<longrightarrow> P a (left + 1) right p)) \<and>
@@ -25,43 +23,16 @@ theorem part1_induct': "(\<forall>a left right p.
   apply (induct rule: part1.induct) by blast
 setup {* add_hoare_induct_rule (@{term part1}, @{thm part1_induct'}) *}
 
-theorem part1_permutes [hoare_triple]:
+declare part1.simps [sep_proc_defs]
+setup {* add_rewrite_rule_cond @{thm Quicksort_Func.part1.simps}
+  [with_filt (size1_filter "l"), with_filt (size1_filter "r")] *}
+lemma part1_to_fun [hoare_triple]:
   "<p \<mapsto>\<^sub>a xs * \<up>(r < length xs)>
    part1 p l r a
-   <\<lambda>rs. \<exists>\<^sub>Axs'. p \<mapsto>\<^sub>a xs' * \<up>(mset xs' = mset xs)>"
+   <\<lambda>rs. p \<mapsto>\<^sub>a snd (Quicksort_Func.part1 xs l r a) * \<up>(rs = fst (Quicksort_Func.part1 xs l r a))>"
 @proof @hoare_induct @qed
-
-theorem part1_returns_index_in_bounds' [hoare_triple]:
-  "<p \<mapsto>\<^sub>a xs * \<up>(r < length xs)>
-   part1 p l r a
-   <\<lambda>rs. \<exists>\<^sub>Axs'. p \<mapsto>\<^sub>a xs' * \<up>(if r \<le> l then rs = r else l \<le> rs \<and> rs \<le> r)>"
-@proof @hoare_induct @qed
-
-theorem part1_outer_remains [hoare_triple]:
-  "<p \<mapsto>\<^sub>a xs * \<up>(r < length xs)>
-   part1 p l r a
-   <\<lambda>_. \<exists>\<^sub>Axs'. p \<mapsto>\<^sub>a xs' * \<up>(outer_remains xs xs' l r)>"
-@proof @hoare_induct @qed
-
-theorem part1_partitions1 [hoare_triple]:
-  "<p \<mapsto>\<^sub>a xs * \<up>(r < length xs)>
-   part1 p l r a
-   <\<lambda>rs. \<exists>\<^sub>Axs'. p \<mapsto>\<^sub>a xs' * \<up>(\<forall>i. l \<le> i \<longrightarrow> i < rs \<longrightarrow> xs' ! i \<le> a)>"
-@proof @hoare_induct @qed
-
-theorem part1_partitions2 [hoare_triple]:
-  "<p \<mapsto>\<^sub>a xs * \<up>(r < length xs)>
-   part1 p l r a
-   <\<lambda>rs. \<exists>\<^sub>Axs'. p \<mapsto>\<^sub>a xs' * \<up>(\<forall>i. rs < i \<longrightarrow> i \<le> r \<longrightarrow> xs' ! i \<ge> a)>"
-@proof @hoare_induct @qed
-
 declare part1.simps [sep_proc_defs del]
-
-theorem part1_returns_index_in_bounds [hoare_triple]:
-  "<p \<mapsto>\<^sub>a xs * \<up>(r < length xs) * \<up>(l \<le> r)>
-   part1 p l r a
-   <\<lambda>rs. \<exists>\<^sub>Axs'. p \<mapsto>\<^sub>a xs' * \<up>(l \<le> rs) * \<up>(rs \<le> r)>" by auto2
-setup {* del_prfstep_thm @{thm part1_returns_index_in_bounds'} *}
+setup {* del_prfstep_thm @{thm Quicksort_Func.part1.simps} *}
 
 (* Partition function. *)
 definition partition :: "nat array \<Rightarrow> nat \<Rightarrow> nat \<Rightarrow> nat Heap" where
@@ -70,122 +41,70 @@ definition partition :: "nat array \<Rightarrow> nat \<Rightarrow> nat \<Rightar
      middle \<leftarrow> part1 a left (right - 1) pivot;
      v \<leftarrow> Array.nth a middle;
      m \<leftarrow> return (if (v \<le> pivot) then (middle + 1) else middle);
-     comment (\<exists>\<^sub>Axs. a \<mapsto>\<^sub>a xs *
-              \<up>(\<forall>i. left \<le> i \<and> i < m \<longrightarrow> xs ! i \<le> pivot) *
-              \<up>(\<forall>i. m \<le> i \<and> i < right - 1 \<longrightarrow> xs ! i \<ge> pivot) *
-              \<up>(xs ! right = pivot));
      swap a m right;
      return m
    }"
+
 declare partition_def [sep_proc_defs]
-
-theorem partition_basics [hoare_triple]:
+setup {* add_rewrite_rule @{thm Quicksort_Func.partition_def} *}
+lemma partition_to_fun [hoare_triple]:
   "<a \<mapsto>\<^sub>a xs * \<up>(l < r) * \<up>(r < length xs)>
    partition a l r
-   <\<lambda>rs. \<exists>\<^sub>Axs'. a \<mapsto>\<^sub>a xs' * \<up>(outer_remains xs xs' l r) * \<up>(mset xs' = mset xs) * \<up>(l \<le> rs \<le> r)>" by auto2
-
-theorem partition_partitions [hoare_triple]:
-  "<a \<mapsto>\<^sub>a xs * \<up>(l < r) * \<up>(r < length xs)>
-   partition a l r
-   <\<lambda>rs. \<exists>\<^sub>Axs'. a \<mapsto>\<^sub>a xs' * \<up>(\<forall>x\<in>set (sublist' l rs xs'). x \<le> xs' ! rs) *
-              \<up>(\<forall>x\<in>set (sublist' (rs + 1) (r + 1) xs'). xs' ! rs \<le> x)>" by auto2
+   <\<lambda>rs. a \<mapsto>\<^sub>a snd (Quicksort_Func.partition xs l r) * \<up>(rs = fst (Quicksort_Func.partition xs l r))>" by auto2
+declare partition_def [sep_proc_defs del]
+setup {* del_prfstep_thm @{thm Quicksort_Func.partition_def} *}
 
 (* Quicksort function *)
 function quicksort :: "nat array \<Rightarrow> nat \<Rightarrow> nat \<Rightarrow> unit Heap" where
   "quicksort a left right =
-     (if left < right then
-        do {
-          pivot \<leftarrow> partition a left right;
-          pivot \<leftarrow> assert (\<lambda>x. left \<le> x \<and> x \<le> right) pivot;
-          comment (\<up>(if pivot > 0 then pivot = 1 + (pivot - 1) else pivot = 0));
-          comment (\<exists>\<^sub>Axs. a \<mapsto>\<^sub>a xs * \<up>(left < length xs) * \<up>(pivot - 1 < length xs));
-          quicksort a left (pivot - 1);
-          comment (\<exists>\<^sub>Axs. a \<mapsto>\<^sub>a xs * \<up>(pivot + 1 \<ge> right \<or> pivot + 1 < length xs));
-          quicksort a (pivot + 1) right
-        }
+     (if left < right then do {
+        pivot \<leftarrow> partition a left right;
+        pivot \<leftarrow> assert (\<lambda>x. left \<le> x \<and> x \<le> right) pivot;
+        quicksort a left (pivot - 1);
+        quicksort a (pivot + 1) right
+      }
      else return ())"
-  by pat_completeness auto
+  by auto
   termination by (relation "measure (\<lambda>(a, l, r). (r - l))") auto
 
-declare quicksort.simps [sep_proc_defs]
-
 theorem quicksort_induct': "(\<forall>arr left right.
-    ((left < right \<longrightarrow> (\<forall>p. left \<le> p \<le> right \<longrightarrow> P arr left (p - 1))) \<and>
-     (left < right \<longrightarrow> (\<forall>p. left \<le> p \<le> right \<longrightarrow> P arr (p + 1) right))) \<longrightarrow> P arr left right) \<Longrightarrow>
+    ((left < right \<longrightarrow> (\<forall>p. left \<le> p \<longrightarrow> p \<le> right \<longrightarrow> P arr left (p - 1))) \<and>
+     (left < right \<longrightarrow> (\<forall>p. left \<le> p \<longrightarrow> p \<le> right \<longrightarrow> P arr (p + 1) right))) \<longrightarrow> P arr left right) \<Longrightarrow>
     P (arr::nat array) (left::nat) (right::nat)"
-  apply (induct rule: quicksort.induct) by (metis closed_interval_def)
+  by (induct rule: quicksort.induct) metis
 setup {* add_hoare_induct_rule (@{term quicksort}, @{thm quicksort_induct'}) *}
+
+declare quicksort.simps [sep_proc_defs]
+setup {* add_rewrite_rule_cond @{thm Quicksort_Func.quicksort.simps}
+  [with_filt (size1_filter "l"), with_filt (size1_filter "r")] *}
 
 theorem quicksort_trivial [hoare_triple]:
   "<a \<mapsto>\<^sub>a xs * \<up>(l \<ge> r)>
    quicksort a l r
-   <\<lambda>_. \<exists>\<^sub>Axs'. a \<mapsto>\<^sub>a xs' * \<up>(xs' = xs)>" by auto2
+   <\<lambda>_. a \<mapsto>\<^sub>a Quicksort_Func.quicksort xs l r>" by auto2
 
-theorem quicksort_outer_remains [hoare_triple]:
+theorem quicksort_to_fun [hoare_triple]:
   "<a \<mapsto>\<^sub>a xs * \<up>(l < length xs) * \<up>(r < length xs)>
    quicksort a l r
-   <\<lambda>rs. \<exists>\<^sub>Axs'. a \<mapsto>\<^sub>a xs' * \<up>(outer_remains xs xs' l r)>"
-@proof @hoare_induct @qed
-
-theorem quicksort_permutes' [hoare_triple]:
-  "<a \<mapsto>\<^sub>a xs * \<up>(l < length xs) * \<up>(r < length xs)>
-   quicksort a l r
-   <\<lambda>rs. \<exists>\<^sub>Axs'. a \<mapsto>\<^sub>a xs' * \<up>(mset xs' = mset xs)>"
-@proof @hoare_induct @qed
+   <\<lambda>_. a \<mapsto>\<^sub>a Quicksort_Func.quicksort xs l r>"
+@proof @hoare_induct
+  @contradiction
+  @case "l < r" @with
+    @have "l < r \<and> r < length xs"
+    @let "p = fst (Quicksort_Func.partition xs l r)"
+    @have "p \<ge> l \<and> p \<le> r"
+    @case "p + 1 \<ge> r"
+    @have "p - 1 < length xs"
+    @case "l \<ge> p - 1"
+  @end
+@qed
 
 declare quicksort.simps [sep_proc_defs del]
-theorem quicksort_permutes [hoare_triple]:
-  "<a \<mapsto>\<^sub>a xs * \<up>(l < length xs) * \<up>(r < length xs)>
-   quicksort a l r
-   <\<lambda>rs. \<exists>\<^sub>Axs'. a \<mapsto>\<^sub>a xs' * \<up>(mset (sublist' l (r+1) xs') = mset (sublist' l (r+1) xs))>" by auto2
-setup {* del_prfstep_thm @{thm quicksort_permutes'} *}
-
-(* Outer remains theorems particular to quicksort. *)
-theorem outer_remains_eqs1: "outer_remains xs xs' (l+1) r \<Longrightarrow>
-  xs' ! l = xs ! l \<and> sublist' x l xs' = sublist' x l xs" by auto2
-
-theorem outer_remains_eqs2: "outer_remains xs xs' l r \<Longrightarrow>
-  xs' ! (r+1) = xs ! (r+1) \<and> sublist' (r+2) y xs' = sublist' (r+2) y xs" by auto2
-
-setup {* fold (add_rewrite_rule_bidir o conj_left_th) [@{thm outer_remains_eqs1}, @{thm outer_remains_eqs2}] *}
-setup {* fold (add_rewrite_rule_bidir o conj_right_th) [@{thm outer_remains_eqs1}, @{thm outer_remains_eqs2}] *}
-
-(* Sortedness of lists of form x @ [pivot] @ y. *)
-setup {* add_rewrite_rule @{thm sorted_append} *}
-theorem sorted_pivoted_list [forward]: "sorted (sublist' (pivot + 1) r xs) \<Longrightarrow> sorted (sublist' l pivot xs) \<Longrightarrow>
-  \<forall>x\<in>set (sublist' l pivot xs). x \<le> xs ! pivot \<Longrightarrow> \<forall>y\<in>set (sublist' (pivot + 1) r xs). xs ! pivot \<le> y \<Longrightarrow>
-  l \<le> pivot \<Longrightarrow> pivot < r \<Longrightarrow> r \<le> length xs \<Longrightarrow> sorted (sublist' l r xs)"
-@proof
-  @have "sublist' pivot r xs = xs ! pivot # sublist' (pivot + 1) r xs" @then
-  @case "pivot = 0" @then
-  @have "sublist' l r xs = sublist' l pivot xs @ sublist' pivot r xs"
-@qed
-setup {* del_prfstep_thm @{thm sorted_append} *}
-
-theorem sorted_pivoted_list' [forward]: "sorted (sublist' 1 r xs) \<Longrightarrow>
-  \<forall>y\<in>set (sublist' 1 r xs). xs ! 0 \<le> y \<Longrightarrow> r \<le> length xs \<Longrightarrow> sorted (sublist' 0 r xs)"
-@proof
-  @contradiction
-  @have "sublist' 0 r xs = xs ! 0 # sublist' 1 r xs"
-@qed
-
-declare quicksort.simps [sep_proc_defs]
-
-setup {* add_gen_prfstep ("quicksort_case",
-  [WithTerm @{term_pat "quicksort ?a ?l ?r"},
-   CreateCase @{term_pat "(?l::nat) < ?r"}]) *}
-
-theorem sorted_triv_list:
-  "l \<ge> r \<Longrightarrow> sorted (sublist' l (r + 1) xs)"
-@proof
-  @case "l \<ge> length xs" @then @case "l = r" @then @have "l > r"
-@qed
-setup {* add_forward_prfstep_cond @{thm sorted_triv_list} [with_term "sublist' ?l (?r + 1) ?xs"] *}
-
+setup {* del_prfstep_thm @{thm Quicksort_Func.quicksort.simps} *}
+  
 theorem quicksort_sorts:
   "<a \<mapsto>\<^sub>a xs * \<up>(l < length xs) * \<up>(r < length xs)>
    quicksort a l r
-   <\<lambda>rs. \<exists>\<^sub>Axs'. a \<mapsto>\<^sub>a xs' * \<up>(sorted (sublist' l (r + 1) xs'))>"
-@proof @hoare_induct @qed
+   <\<lambda>rs. \<exists>\<^sub>Axs'. a \<mapsto>\<^sub>a xs' * \<up>(sorted (sublist' l (r + 1) xs'))>" by auto2
 
 end
