HOL/DataStrs/Quicksort_Func.thy
@@ -1,0 +1,184 @@
+theory Quicksort_Func
+imports Reverse_Func
+begin
+
+section {* Outer remains *}
+  
+definition outer_remains :: "'a list \<Rightarrow> 'a list \<Rightarrow> nat \<Rightarrow> nat \<Rightarrow> bool" where [rewrite]:
+  "outer_remains xs xs' l r \<longleftrightarrow> (\<forall>i. i < l \<or> r < i \<longrightarrow> xs ! i = xs' ! i)"
+
+lemma outer_remainsD1: "outer_remains xs xs' l r \<Longrightarrow> i < l \<Longrightarrow> xs ! i = xs' ! i" by auto2
+setup {* add_forward_prfstep_cond @{thm outer_remainsD1} [with_term "?xs' ! ?i"] *}
+
+lemma outer_remainsD2: "outer_remains xs xs' l r \<Longrightarrow> r < i \<Longrightarrow> xs ! i = xs' ! i" by auto2
+setup {* add_forward_prfstep_cond @{thm outer_remainsD2} [with_term "?xs' ! ?i"] *}
+setup {* del_prfstep_thm_str "@eqforward" @{thm outer_remains_def} *}
+
+section {* part1 function *}  
+
+function part1 :: "('a::linorder) list \<Rightarrow> nat \<Rightarrow> nat \<Rightarrow> 'a \<Rightarrow> (nat \<times> 'a list)" where
+  "part1 xs l r a = (
+     if r \<le> l then (r, xs)
+     else if xs ! l \<le> a then part1 xs (l + 1) r a
+     else part1 (list_swap xs l r) l (r - 1) a)"
+  by auto
+  termination by (relation "measure (\<lambda>(_,l,r,_). r - l)") auto
+setup {* add_rewrite_rule_cond @{thm part1.simps} [with_filt (size1_filter "l"), with_filt (size1_filter "r")] *}
+setup {* register_wellform_data ("part1 xs l r a", ["r < length xs"]) *}
+
+lemma nat_sub3 [rewrite]: "(r::nat) - (l + 1) = r - l - 1" by simp
+
+lemma part1_basic: "r < length xs \<Longrightarrow> xs' = snd (part1 xs l r a) \<Longrightarrow>
+  length xs' = length xs \<and> outer_remains xs xs' l r \<and> mset xs' = mset xs"
+@proof
+  @let "d = r - l"
+  @strong_induct d arbitrary l r xs
+  @case "r \<le> l"
+  @case "xs ! l \<le> a" @with @apply_induct_hyp "d - 1" "l + 1" r xs @end
+  @apply_induct_hyp "d - 1" l "r - 1" "list_swap xs l r"
+@qed
+setup {* add_forward_prfstep_cond @{thm part1_basic} [with_term "?xs'"] *}
+
+lemma part1_returns_index_in_bounds:
+  "r < length xs \<Longrightarrow> rs = fst (part1 xs l r a) \<Longrightarrow> l \<le> r \<Longrightarrow> l \<le> rs \<and> rs \<le> r"
+@proof
+  @let "d = r - l"
+  @strong_induct d arbitrary l r xs
+  @case "r \<le> l"
+  @case "xs ! l \<le> a" @with @apply_induct_hyp "d - 1" "l + 1" r xs @end
+  @apply_induct_hyp "d - 1" l "r - 1" "list_swap xs l r"
+@qed
+setup {* add_forward_prfstep_cond @{thm part1_returns_index_in_bounds} [with_term "?rs"] *}
+
+lemma part1_partitions1:
+  "r < length xs \<Longrightarrow> rs = fst (part1 xs l r a) \<Longrightarrow> xs' = snd (part1 xs l r a) \<Longrightarrow>
+   l \<le> i \<Longrightarrow> i < rs \<Longrightarrow> xs' ! i \<le> a"
+@proof
+  @let "d = r - l"
+  @strong_induct d arbitrary l r xs i
+  @case "r \<le> l"
+  @case "xs ! l \<le> a" @with
+    @case "l + 1 \<le> i" @with @apply_induct_hyp "d - 1" "l + 1" r xs i @end
+    @have "l < l + 1"
+  @end
+  @apply_induct_hyp "d - 1" l "r - 1" "list_swap xs l r"
+@qed
+setup {* add_forward_prfstep_cond @{thm part1_partitions1} [with_term "?xs' ! ?i"] *}
+
+lemma part1_partitions2:
+  "r < length xs \<Longrightarrow> rs = fst (part1 xs l r a) \<Longrightarrow> xs' = snd (part1 xs l r a) \<Longrightarrow>
+   rs < i \<Longrightarrow> i \<le> r \<Longrightarrow> xs' ! i \<ge> a"
+@proof
+  @let "d = r - l"
+  @strong_induct d arbitrary l r xs i
+  @case "r \<le> l"
+  @case "xs ! l \<le> a" @with @apply_induct_hyp "d - 1" "l + 1" r xs @end
+  @case "i \<le> r - 1" @with @apply_induct_hyp "d - 1" l "r - 1" "list_swap xs l r" i @end
+  @have "r - 1 < length xs"
+@qed
+setup {* add_forward_prfstep_cond @{thm part1_partitions2} [with_term "?xs' ! ?i"] *}
+
+setup {* del_prfstep_thm @{thm part1.simps} *}
+
+section {* Paritition function *}
+
+definition partition :: "('a::linorder list) \<Rightarrow> nat \<Rightarrow> nat \<Rightarrow> (nat \<times> 'a list)" where [rewrite]:
+  "partition xs l r = (
+    let p = xs ! r;
+      m = fst (part1 xs l (r - 1) p);
+      xs' = snd (part1 xs l (r - 1) p);
+      m' = if xs' ! m \<le> p then m + 1 else m
+    in
+      (m', list_swap xs' m' r))"
+setup {* register_wellform_data ("partition xs l r", ["l < r", "r < length xs"]) *}
+
+lemma partition_return_in_bounds:
+  "l < r \<Longrightarrow> r < length xs \<Longrightarrow> rs = fst (partition xs l r) \<Longrightarrow> l \<le> rs \<and> rs \<le> r"
+@proof @have "r - 1 < length xs" @qed
+setup {* add_forward_prfstep_cond @{thm partition_return_in_bounds} [with_term "?rs"] *}
+
+lemma partition_basic:
+  "l < r \<Longrightarrow> r < length xs \<Longrightarrow> xs' = snd (partition xs l r) \<Longrightarrow>
+   length xs' = length xs \<and> outer_remains xs xs' l r \<and> mset xs' = mset xs"
+@proof @have "r - 1 < length xs" @qed
+setup {* add_forward_prfstep_cond @{thm partition_basic} [with_term "?xs'"] *}
+
+lemma partition_partitions1:
+  "l < r \<Longrightarrow> r < length xs \<Longrightarrow> rs = fst (partition xs l r) \<Longrightarrow> xs' = snd (partition xs l r) \<Longrightarrow>
+   i \<ge> l \<Longrightarrow> i < rs \<Longrightarrow> xs' ! i \<le> xs' ! rs"
+@proof
+  @have "r - 1 < length xs"
+  @let "p = xs ! r"
+  @let "xs'' = snd (part1 xs l (r - 1) p)"
+  @have "xs'' ! r = p"
+  @have (@rule) "\<forall>j. j \<ge> l \<longrightarrow> j < rs \<longrightarrow> xs'' ! j \<le> p"
+@qed
+setup {* add_forward_prfstep_cond @{thm partition_partitions1} [with_term "?xs' ! ?i"] *}
+
+lemma partition_partitions2:
+  "l < r \<Longrightarrow> r < length xs \<Longrightarrow> rs = fst (partition xs l r) \<Longrightarrow> xs' = snd (partition xs l r) \<Longrightarrow>
+   i \<ge> rs + 1 \<Longrightarrow> i \<le> r \<Longrightarrow> xs' ! i \<ge> xs' ! rs"
+@proof
+  @have "r - 1 < length xs" @have "r - 1 < r"
+  @let "p = xs ! r"
+  @let "m = fst (part1 xs l (r - 1) p)"
+  @let "xs'' = snd (part1 xs l (r - 1) p)"
+  @have "xs'' ! r = p"
+  @have (@rule) "\<forall>j. rs \<le> j \<longrightarrow> j < r - 1 \<longrightarrow> xs'' ! j \<ge> p" @with
+    @case "m = j" @end
+@qed
+setup {* add_forward_prfstep_cond @{thm partition_partitions2} [with_term "?xs' ! ?i"] *}
+
+setup {* del_prfstep_thm @{thm partition_def} *}
+
+function quicksort :: "('a::linorder) list \<Rightarrow> nat \<Rightarrow> nat \<Rightarrow> 'a list" where
+  "quicksort xs l r = (
+    if l < r \<and> r < length xs then
+      let p = fst (partition xs l r);
+        xs1 = snd (partition xs l r);
+        xs2 = quicksort xs1 l (p - 1)
+      in
+        quicksort xs2 (p + 1) r
+    else xs)"
+  by auto
+  termination apply (relation "measure (\<lambda>(a, l, r). (r - l))")
+  apply auto
+  apply (smt Suc_diff_Suc Suc_le_lessD diff_is_0_eq le_diff_iff less_imp_diff_less less_imp_le
+             not_less partition_return_in_bounds)
+  by (simp add: diff_less_mono2 less_Suc_eq_le partition_return_in_bounds)
+
+setup {* add_rewrite_rule_cond @{thm quicksort.simps}
+  [with_filt (size1_filter "l"), with_filt (size1_filter "r")] *}
+setup {* register_wellform_data ("quicksort xs l r", ["l < length xs", "r < length xs"]) *}
+
+lemma diff_less_mono [backward1]: "a \<ge> c \<Longrightarrow> (a::nat) < b \<Longrightarrow> a - c < b - c" by simp
+
+lemma quicksort_trivial [rewrite]:
+  "r < length xs \<Longrightarrow> l \<ge> r \<Longrightarrow> quicksort xs l r = xs" by auto2
+
+lemma quicksort_basic:
+  "l < length xs \<Longrightarrow> r < length xs \<Longrightarrow> xs3 = quicksort xs l r \<Longrightarrow>
+   length xs3 = length xs \<and> mset xs3 = mset xs \<and> outer_remains xs xs3 l r"
+@proof
+  @let "d = r - l"
+  @strong_induct d arbitrary l r xs xs3
+  @let "p = fst (partition xs l r)"
+  @let "xs1 = snd (partition xs l r)"
+  @let "xs2 = quicksort xs1 l (p - 1)"
+  @case "l \<ge> r"
+  @have "p - 1 < length xs"
+  @have "length xs2 = length xs1 \<and> mset xs2 = mset xs1 \<and> outer_remains xs1 xs2 l r" @with
+    @case "p - 1 \<le> l" @then
+    @have "p - 1 - l < r - l" @with @have "p - 1 < r" @end
+    @apply_induct_hyp "p - 1 - l" l "p - 1" xs1
+  @end
+  @have "length xs3 = length xs2 \<and> mset xs3 = mset xs2 \<and> outer_remains xs2 xs3 l r" @with
+    @case "p + 1 \<ge> r" @then
+    @have "r - (p + 1) < r - l"
+    @apply_induct_hyp "r - (p + 1)" "p + 1" r xs2
+  @end
+@qed
+setup {* add_forward_prfstep_cond @{thm quicksort_basic} [with_term "?xs3.0"] *}
+setup {* del_prfstep_thm @{thm quicksort.simps} *}
+
+end
