HOL/DataStrs/Quicksort_Func2.thy
@@ -1,0 +1,101 @@
+theory Quicksort_Func2
+imports Quicksort_Func "../SepLogic/More_Lists"
+begin
+
+lemma quicksort_permutes:
+  "l < length xs \<Longrightarrow> r < length xs \<Longrightarrow> xs' = quicksort xs l r \<Longrightarrow>
+   mset (sublist' l (r + 1) xs') = mset (sublist' l (r + 1) xs)" by auto2
+setup {* add_forward_prfstep_cond @{thm quicksort_permutes} [with_term "?xs'"] *}
+
+(* Outer remains theorems particular to quicksort. *)
+lemma outer_remains_eqs1:
+  "outer_remains xs xs' (l+1) r \<Longrightarrow> length xs = length xs' \<Longrightarrow>
+   xs' ! l = xs ! l \<and> sublist' x l xs' = sublist' x l xs" by auto2
+
+lemma outer_remains_eqs2:
+  "outer_remains xs xs' l r \<Longrightarrow> length xs = length xs' \<Longrightarrow>
+   xs' ! (r+1) = xs ! (r+1) \<and> sublist' (r+2) y xs' = sublist' (r+2) y xs" by auto2
+
+setup {* fold (add_rewrite_rule_bidir o conj_left_th) [@{thm outer_remains_eqs1}, @{thm outer_remains_eqs2}] *}
+setup {* fold (add_rewrite_rule_bidir o conj_right_th) [@{thm outer_remains_eqs1}, @{thm outer_remains_eqs2}] *}
+
+(* Sortedness of lists of form x @ [pivot] @ y. *)
+setup {* add_rewrite_rule @{thm sorted_append} *}
+lemma sorted_pivoted_list [forward]: "sorted (sublist' (p + 1) r xs) \<Longrightarrow> sorted (sublist' l p xs) \<Longrightarrow>
+  \<forall>x\<in>set (sublist' l p xs). x \<le> xs ! p \<Longrightarrow> \<forall>y\<in>set (sublist' (p + 1) r xs). xs ! p \<le> y \<Longrightarrow>
+  l \<le> p \<Longrightarrow> p < r \<Longrightarrow> r \<le> length xs \<Longrightarrow> sorted (sublist' l r xs)"
+@proof
+  @have "sublist' p r xs = xs ! p # sublist' (p + 1) r xs" @then
+  @case "p = 0" @then
+  @have "sublist' l r xs = sublist' l p xs @ sublist' p r xs"
+@qed
+setup {* del_prfstep_thm @{thm sorted_append} *}
+
+lemma sorted_triv_list: "l \<ge> r \<Longrightarrow> sorted (sublist' l (r + 1) xs)"
+@proof
+  @case "l \<ge> length xs" @then @case "l = r" @then @have "l > r"
+@qed
+setup {* add_forward_prfstep_cond @{thm sorted_triv_list} [with_term "sublist' ?l (?r + 1) ?xs"] *}
+
+setup {* add_rewrite_rule_cond @{thm quicksort.simps}
+  [with_filt (size1_filter "l"), with_filt (size1_filter "r")] *}
+
+lemma quicksort_sorts:
+  "l < length xs \<Longrightarrow> r < length xs \<Longrightarrow> sorted (sublist' l (r + 1) (quicksort xs l r))"
+@proof
+  @let "d = r - l"
+  @strong_induct d arbitrary l r xs
+  @let "p = fst (partition xs l r)"
+  @let "xs1 = snd (partition xs l r)"
+  @let "xs2 = quicksort xs1 l (p - 1)"
+  @let "xs3 = quicksort xs l r"
+  @case "l \<ge> r"
+  @have "l < r \<and> r < length xs"
+  @have "p - 1 < length xs"
+  @case "l < p - 1" @with
+    @case "p = 0"
+    @case "p + 1 < r" @with
+      @have "p + 1 < length xs"
+      @have "sorted (sublist' l p xs3)" @with
+        @have "p - 1 - l < r - l" @with @have "p - 1 < r" @end
+        @apply_induct_hyp "p - 1 - l" l "p - 1" xs1
+      @end
+      @have "sorted (sublist' (p + 1) (r + 1) xs3)" @with
+        @have "r - (p + 1) < r - l"
+        @apply_induct_hyp "r - (p + 1)" "p + 1" r xs2
+      @end
+      @have "sorted (sublist' l p xs3)"
+      @have "\<forall>x\<in>set (sublist' l p xs3). x \<le> xs3 ! p"
+      @have "\<forall>x\<in>set (sublist' (p + 1) (r + 1) xs3). x \<ge> xs3 ! p"
+    @end
+    @have "sorted (sublist' l p xs3)" @with
+      @have "p - 1 - l < r - l" @with @have "p - 1 < r" @end
+      @apply_induct_hyp "p - 1 - l" l "p - 1" xs1
+    @end
+    @have "sorted (sublist' (p + 1) (r + 1) xs3)"
+    @have "\<forall>x\<in>set (sublist' l p xs3). x \<le> xs3 ! p"
+    @have "\<forall>x\<in>set (sublist' (p + 1) (r + 1) xs3). x \<ge> xs3 ! p"
+  @end
+  @case "p + 1 < r" @with
+    @have "p + 1 < length xs"
+    @have "sorted (sublist' (p + 1) (r + 1) xs3)" @with
+      @have "r - (p + 1) < r - l"
+      @apply_induct_hyp "r - (p + 1)" "p + 1" r xs2
+    @end
+    @have "sorted (sublist' l p xs3)" @with
+      @case "p = 0" @have "p = p - 1 + 1" @end
+    @have "sorted (sublist' (p + 1) (r + 1) xs3)"
+    @have "\<forall>x\<in>set (sublist' l p xs3). x \<le> xs3 ! p"
+    @have "\<forall>x\<in>set (sublist' (p + 1) (r + 1) xs3). x \<ge> xs3 ! p"
+  @end
+  @have "sorted (sublist' l p xs3)" @with
+    @case "p = 0" @have "p = p - 1 + 1" @end
+  @have "sorted (sublist' (p + 1) (r + 1) xs3)"
+  @have "\<forall>x\<in>set (sublist' l p xs3). x \<le> xs3 ! p"
+  @have "\<forall>x\<in>set (sublist' (p + 1) (r + 1) xs3). x \<ge> xs3 ! p"  
+@qed
+setup {* add_forward_prfstep_cond @{thm quicksort_sorts} [with_term "quicksort ?xs ?l ?r"] *}
+
+setup {* del_prfstep_thm @{thm quicksort.simps} *}
+
+end
